ModularEngine/src/LogicEngine.FStar/coredkal2.fst
@@ -1,0 +1,250 @@
+(*
+// *********************************************************
+//
+//    Copyright (c) Microsoft. All rights reserved.
+//    This code is licensed under the Apache License, Version 2.0.
+//    THIS CODE IS PROVIDED *AS IS* WITHOUT WARRANTY OF
+//    ANY KIND, EITHER EXPRESS OR IMPLIED, INCLUDING ANY
+//    IMPLIED WARRANTIES OF FITNESS FOR A PARTICULAR
+//    PURPOSE, MERCHANTABILITY, OR NON-INFRINGEMENT.
+//
+// *********************************************************
+*)
+
+(************************************************)
+(* build:                                       *)
+(* fstar typeHeaders.fst types.fst coredkal.fst *)
+(* or:                                          *)
+(* make coredkal                                *)
+(************************************************)
+
+module CoreDKAL
+
+(********************)
+(* Type definitions *)
+(********************)
+
+open Types
+open Util
+open Typing
+open Subst
+
+val memInfostrate : i:term -> k:infostrate -> b:bool{b=true <=> (In i k)}
+(* impl todo *)
+  
+(******************************)
+(* Trusted external functions *)
+(******************************)
+(* Queries to external databases i.e., Substrate *)
+type SubstrateSays :: substrate => ISubstrateQueryTerm => E
+val check_substrate : s:substrate -> q:ISubstrateQueryTerm -> b:bool{b=true => SubstrateSays s q}
+(* impl todo *)
+
+(***********************)
+(* Inductive judgments *)
+(***********************)
+logic function WithPrefix : prefix -> term -> term 
+assume forall (i:term). (WithPrefix [] i) = i
+assume forall (p:term) (pfx:prefix) (i:term). (WithPrefix (p::pfx) i) = (WithPrefix pfx (App SaidInfon [p; i]))
+
+logic function WithPrefixL : prefix -> list term -> list term
+assume forall (pfx:prefix). (WithPrefixL pfx []) = []
+assume forall (pfx:prefix) (t:term) (tl:list term). (WithPrefixL pfx (t::tl)) = ((WithPrefix pfx t)::(WithPrefixL pfx tl))
+assume forall (p:term) (pfx:prefix) (i:term). (WithPrefix (p::pfx) i) = (App SaidInfon [p; (WithPrefix pfx i)])
+
+val withPrefix: pfx:prefix -> i:term -> j:term{j=(WithPrefix pfx i)}
+let rec withPrefix pfx i = match pfx with 
+  | [] -> i
+  | p::pfx' -> (withPrefix pfx' (App SaidInfon [p; i]))
+
+val stripPrefix: i:term -> pref:prefix -> j:term{(WithPrefix pref j)=i}
+(* stripPrefix is a partial function *)
+
+val withPrefixL: pfx:prefix -> i:list term -> j:list term{j=(WithPrefixL pfx i)}
+
+type entails :: substrate => infostrate => varDecl => term => P =
+  | Entails_Emp : 
+       S:substrate -> K:infostrate -> G:varDecl
+    -> pref:prefix
+    -> WF S K G
+    -> types G (WithPrefix pref (App EmptyInfon [])) Infon
+    -> entails S K G (WithPrefix pref (App EmptyInfon []))
+
+  | Entails_Hyp_Knowledge : 
+       S:substrate -> K:infostrate -> G:varDecl
+    -> i:term{In i K}
+    -> WF S K G
+    -> entails S K G i
+
+  | Entails_Hyp_Substrate : 
+       S:substrate -> K:infostrate -> G:varDecl
+    -> q:ISubstrateQueryTerm{SubstrateSays S q}     (* Eventually, we get a signature from the DB about this fact *)
+    -> WF S K G
+    -> entails S K G (App AsInfon [(SubstrateQueryTerm q)])
+
+  | Entails_Q_Intro : 
+       S:substrate -> K:infostrate -> G:varDecl
+    -> x:var -> i:term 
+    -> entails S K (x::G) i
+    -> entails S K G (ForallT x i)
+
+  | Entails_Q_Inst : 
+       S:substrate -> K:infostrate -> G:varDecl
+    -> v:var -> i:term -> u:term 
+    -> i':term{Subst i (Update EmptySubst v u) i'}
+    -> entails S K G (ForallT v i)
+    -> types G u v.typ
+    -> entails S K G i'
+
+  | Entails_And_Intro : 
+       S:substrate -> K:infostrate -> G:varDecl
+    -> ilist:list term -> pref:prefix
+    -> MapL term (entails S K G) (WithPrefixL pref ilist)
+    -> entails S K G (WithPrefix pref (App AndInfon ilist))
+
+  | Entails_And_Intro2 : (* Simpler version with binary And *)
+       S:substrate -> K:infostrate -> G:varDecl
+    -> i:term -> j:term -> pref:prefix
+    -> entails S K G (WithPrefix pref i)
+    -> entails S K G (WithPrefix pref j)
+    -> entails S K G (WithPrefix pref (App AndInfon [i;j]))
+
+  | Entails_And_Elim : 
+       S:substrate -> K:infostrate -> G:varDecl
+    -> ilist:list term -> i:term{In i ilist} -> pref:prefix
+    -> entails S K G (WithPrefix pref (App AndInfon ilist))
+    -> entails S K G (WithPrefix pref i)
+
+  | Entails_W_Imp_Intro : 
+       S:substrate -> K:infostrate -> G:varDecl
+    -> i:term -> j:term -> pref:prefix
+    -> entails S K G (WithPrefix pref j)
+    -> types G i Infon
+    -> entails S K G (WithPrefix pref (App ImpliesInfon [i; j]))
+
+  | Entails_Imp_Elim : 
+       S:substrate -> K:infostrate -> G:varDecl
+    -> i:term -> j:term -> pref:list term
+    -> entails S K G (WithPrefix pref i)
+    -> entails S K G (WithPrefix pref (App ImpliesInfon [i;j]))
+    -> entails S K G (WithPrefix pref j)
+
+  | Entails_Alpha :
+      S:substrate -> K:infostrate -> G:varDecl
+    -> x:var -> i:term -> y:var -> i':term{Subst i (Update EmptySubst x (Var y)) i'}
+    -> entails S K G (ForallT y i')
+    -> entails S K G (ForallT x i)
+
+(*************************)
+(* Derivation algorithms *)
+(*************************)
+
+(* prove as lemmas *)
+assume forall (s1:substitution) (s2:substitution) (s3:substitution). 
+            Extends s3 s2 && Extends s2 s1 => Extends s3 s1
+assume forall (pref:prefix) (pref':prefix) (t:term) (t':term) (s:substitution). 
+             (SubstList pref s pref' && Subst t s t')
+            => Subst (WithPrefix pref t) s (WithPrefix pref' t')
+
+type result :: _ = 
+    (fun (s:substrate) (k:infostrate) (g:varDecl) (s3:substitution) (pref:prefix) (goal:term) => 
+        (goal':term{Subst goal s3 goal'} * pref':prefix{SubstList pref s3 pref'} * entails s k g (WithPrefix pref' goal')))
+        (* (goal':term{Subst goal s4 goal'} * pref':prefix{SubstList pref s4 pref'} * entails s k g (WithPrefix pref' goal'))) *)
+
+val doDerive:   S:substrate 
+             -> K:infostrate 
+             -> G:varDecl
+             -> U:varDecl             (* Variables available for unification in goal *)
+     	     -> s1:substitution
+             -> pref:prefix 
+             -> goal:term
+             -> option (s2:substitution{Extends s2 s1} *
+                          (s3:substitution{Extends s3 s2} ->  (goal':term{Subst goal s3 goal'} *
+                                                                 pref':prefix{SubstList pref s3 pref'} *
+                                                                 entails S K G (WithPrefix pref' goal'))))
+
+val unify: u:varDecl 
+        -> s1:substitution
+        -> i:term    
+        -> goal:term (* u subsetof (freevars goal) *)
+        -> option (s2:substitution{Extends s2 s1})
+(* ad hoc implementation of unification
+     informally, only variables in u are available for unification.
+*)
+
+val tryDerive:  S:substrate 
+             -> K:infostrate 
+             -> G:varDecl
+             -> U:varDecl             (* Variables available for unification in goal *)
+     	     -> s1:substitution
+             -> pref:prefix 
+             -> i:term{In i K}
+             -> goal:term
+             -> option (s2:substitution{Extends s2 s1} *
+                          (s3:substitution{Extends s3 s2} -> (goal':term{Subst goal s3 goal'} *
+                                                                pref':prefix{SubstList pref s3 pref'} *
+                                                                entails S K G (WithPrefix pref' goal'))))
+let tryDerive s k g u s1 pref i goal = 
+  let pref_goal = withPrefix pref goal in
+    match unify u s1 i pref_goal with 
+      | None -> None
+      | Some s2 -> 
+          let continuation (s3:substitution{Extends s3 s2}) = 
+            let goal' = subst goal s3 in  (* Subst goal s3 goal' *)
+            let pref' = substList pref s3 in  (* SubstList pref s3 pref' *)
+            let pref_goal' = withPrefix pref' goal' in  (* pref_goal'= (WithPrefix pref' goal') *)
+              if (pref_goal':term) = i then 
+                match checkWF s k g with 
+                  | Some pf_wf -> 
+                      let pf = Entails_Hyp_Knowledge s k g i pf_wf in 
+                        ((goal', pref', pf) : 
+                           (goal':term{Subst goal s3 goal'} *
+                              pref':prefix{SubstList pref s3 pref'} *
+                              entails s k g (WithPrefix pref' goal')))
+                  | None -> raise "ill-formed environment"
+              else raise "bad substitution" in 
+            Some (s2, continuation)
+
+(* result S K G s3 pref goal) *)
+let rec doDerive s k g u s1 pref goal = 
+  match map_one k (fun (i:term{In i k}) -> tryDerive s k g u s1 pref i goal) with (* should this be done last? *)
+    | Some result -> Some result
+    | None -> 
+        match goal with 
+          | App AndInfon [goal_i; goal_j] -> 
+              (match doDerive s k g u s1 pref goal_i with 
+                 | None -> None
+                 | Some((s2, mkpf_i)) -> 
+                     match doDerive s k g u s2 pref goal_j with 
+                       | None -> None
+                       | Some((s3, mkpf_j)) -> 
+                           let continuation (s4:substitution{Extends s4 s3}) = 
+                             let goal_i', pref_i', pf_i' = mkpf_i s4 in (* from lemma: Extends s4 s2 *) (* pf_i': entails s k g (WithPrefix pref_i' goal_i') *) 
+                             let goal_j', pref_j', pf_j' = mkpf_j s4 in (* Extends s4 s3, directly *) (* pf_j': entails s k g (WithPrefix pref_j' goal_j') *)
+                               if (pref_i'=pref_j') (* we know: Subst pref s4 pref_i' and  Subst pref s4 pref_j'; but not pref_i'=pref_j' *)
+                               then
+                                 let pf_and = Entails_And_Intro2 s k g goal_i' goal_j' pref_i' pf_i' pf_j' in
+                                 let goal' = App AndInfon [goal_i'; goal_j'] in  (* pf_and: Entails s k g goal'*)
+                                   ((goal', pref_i', pf_and)
+                                      :(goal':term{Subst goal s4 goal'} * pref':prefix{SubstList pref s4 pref'} * entails s k g (WithPrefix pref' goal')))
+                               else raise "bad substitution" in 
+                             Some (s3, continuation))
+                
+          | App SaidInfon [p;j] ->
+              (match doDerive s k g u s1 (p::pref) j with
+                 | Some ((s2, mkpf_j)) ->  (* s2:substitution{Extends s2 s1} * (s3:subst{Extends s3 s2} -> (goal_j':term{Subst goal_j s3 goal_j'} *
+                                              pref_j':prefix{SubstList (p::pref) s3 pref'} *
+                                              entails s k g (WithPrefix pref_j' goal_j'))) *)
+                     let continuation (s3:substitution{Extends s3 s2}) =
+                       let goal_j', pref_j', pf_j' = mkpf_j s3 in (* SubstList (p::pref) s3 pref_j'; we should prove that pref_j' = p'::pref' where (Subst p s3 p') *)
+                         match pref_j' with
+                           | p'::pref' -> (* should prove that (Subst p s3 p') *)
+                               let goal' = App SaidInfon [p'; goal_j'] in
+                                 ((goal', pref', pf_j')
+                                    : (goal':term{Subst goal s3 goal'} * pref':prefix{SubstList pref s3 pref'} * entails s k g (WithPrefix pref' goal')))
+                           | [] -> raise "impos" in (* prove that this case is unreachable by asserting false *) 
+                       Some (s2, continuation))
+
+          | _ -> None (* todo *)
+              
+              
