ModularEngine/src/LogicEngine.FStar/subst.fst
@@ -1,0 +1,175 @@
+module Subst
+open Types
+open Util
+
+(* Axiomatization of sets of variables *)
+logic function Empty : varset
+logic function Singleton : var -> varset
+logic function Union : varset -> varset -> varset
+assume forall (v:var). (In v (Singleton v))
+assume forall (l1:varset) (l2:varset) (v:var). 
+        ((In v l1) || (In v l2)) => (In v (Union l1 l2))
+assume forall (v:var). not(In v Empty)
+(* extern Runtime *) val union : s1:varset -> s2:varset -> s3:varset{(s3 = (Union s1 s2))}
+
+(* Axiomatization of substitutions *)
+logic function EmptySubst : substitution
+logic function Domain : substitution -> varset
+logic function Select : substitution -> var -> term
+logic function Update : substitution -> var -> term -> substitution
+logic function FreeVars : term -> varset
+logic function FreeVarsSubst : substitution -> varset 
+  (* set of variable in both the domain and the range of the map *)
+assume forall (s:substitution) (x:var) (t:term). 
+  (Select (Update s x t) x) = t
+assume forall (s:substitution) (x:var) (y:var) (t:term).
+  (x <> y) => ((Select (Update s x t) y) = (Select s y))
+assume forall (s:substitution) (x:var) (t:term). 
+  Domain (Update s x t) = (Union (Domain s) (Singleton x))
+assume (Domain EmptySubst) = Empty
+
+type Subst :: term => substitution => term => E
+type SubstList :: list term => substitution => list term => E
+
+assume Subst_VarRepl: forall (x:var) (s:substitution).
+        (In x (Domain s)) => ((Subst (Var x) s (Select s x)))
+assume Subst_VarIgnore: forall (x:var) (s:substitution).
+        (not (In x (Domain s))) => (Subst (Var x) s (Var x))
+assume Subst_Const:  (forall (c:constant) (s:substitution). 
+        (Subst (Const c) s (Const c)))
+assume Subst_App: forall (f:func) (args:list term) (args': list term) (s:substitution).
+        (SubstList args s args') =>  (Subst (App f args) s (App f args'))
+assume Subst_forallT: forall (x:var) (t:term) (s:substitution) (t':term). 
+        (not(In x (FreeVarsSubst s)) && Subst t s t') => 
+           (Subst (ForallT x t) s (ForallT x t'))
+assume Subst_forallT_Alpha: forall (x:var) (t:term) (s:substitution) (y:var) (t_yx:term) (t':term). 
+        (not(In y (Union (FreeVarsSubst s) (FreeVars t))) &&
+            (Subst t (Update EmptySubst x (Var y)) t_yx) &&
+            (Subst t_yx s t'))
+        => (Subst (ForallT x t) s (ForallT y t'))
+
+assume SubstList_nil: forall (s:substitution). SubstList [] s []
+assume SubstList_cons: forall (t:term) (t':term) (tl:list term) (tl':list term) (s:substitution). 
+        (Subst t s t' && SubstList tl s tl')
+    <=> (SubstList (t::tl) s (t'::tl'))
+
+
+type Extends :: substitution => substitution => E
+assume forall (s:substitution). Extends s s
+assume forall (s1:substitution) (s2:substitution) (x:var) (t:term). 
+          ((Extends s2 s1) && (Subst t s2 t) && (not(In x (Domain s2))))
+        => Extends (Update s2 x t) s1
+
+
+val emptySubst: unit -> s:substitution{s=EmptySubst}
+  
+val lookupVar : 
+     s:substitution 
+  -> x:var 
+  -> o:option term{((o=None <=> (not (In x (Domain s)))) &&
+                      (forall (t:term). (o=(Some t)) => 
+   			  ((In x (Domain s)) && (t=(Select s x)))))}
+
+val extendSubst : 
+     s:substitution 
+  -> x:var 
+  -> t:term{Subst t s t && not(In x (Domain s))}
+  -> s':substitution{s'=(Update s x t)}
+
+val inDomain : 
+     s:substitution 
+  -> x:var 
+  -> b:bool{b=true <=> In x (Domain s)}
+   
+val inFreevars : 
+     s:substitution 
+  -> x:var 
+  -> b:bool{b=true <=> In x (FreeVarsSubst s)}
+
+(* added *)
+val freeVarsSubst : 
+     s:substitution 
+  -> f:varset{(f = (FreeVarsSubst s))}
+
+val freeVars : 
+     t:term 
+  -> f:varset{(f = (FreeVars t))}
+
+
+(* functions from builders.fs *)
+let _freshVarId = ref 0 (* can't go inside because no inside rec function *)
+
+val freshVar : ty:typ -> s:varset 
+             -> x:var{ not ( In x s ) }
+let rec freshVar ty s =
+  let n = { typ = ty; name = (Concat "fresh" (string_of_any (!_freshVarId))) } in
+   (_freshVarId := !_freshVarId + 1); (* Rk: parenthesis needed *)
+   if not (contains n s) 
+   then n 
+   else freshVar ty s
+     
+(* from term.fst *)	 
+extern reference TranslationToFStar {language="F#";
+                                     dll="TranslationToFStar";
+                                     namespace="";
+                                     classname="TranslationToFStar"}
+extern TranslationToFStar val FStarVarOfIVar : IVar -> Types.var
+extern TranslationToFStar val FStarTermOfITerm : ITerm -> Types.term
+extern TranslationToFStar val FStarSubstitutionOfISubstitution: ISubstitution -> Types.substitution	 
+	 
+(* see term_apply in term.fst *)
+val subst: i:term -> s:substitution -> i':term{Subst i s i'}
+val substList : tl:list term -> s:substitution -> tl':list term{SubstList tl s tl'}
+let rec subst i s = 
+  match i with
+    | Var y -> 
+        (match lookupVar s y with 
+           | None -> Var y
+           | Some t -> t)
+          
+    | Const c -> Const c
+        
+    | App f tl -> App f (substList tl s)
+    
+    | ForallT x t -> (* code taken partially from term.fst *)
+      (* the substitution is not applied to the quantified variable *)
+        let y : (yy:var{not(In yy (Union (FreeVars t) (FreeVarsSubst s)))}) =
+          freshVar x.typ (union (freeVars t) (freeVarsSubst s)) in
+		let ySubst : (ys:substitution{(ys = (Update EmptySubst x (Var y)))}) =
+          extendSubst (emptySubst ()) x (Var y) in
+		let t_yx : (t_yx:term{((Subst t (Update EmptySubst x (Var y)) t_yx))}) =
+          subst t ySubst in
+		let t' : (t':term{(Subst t_yx s t')}) =
+          (subst t_yx s) in
+(*         let res : (res:term{Subst i s res}) = Types.ForallT y t' in  *)
+        let res = Types.ForallT y t' in 
+	let _ = Assume <(Subst i s res)> () in
+		res
+		
+(*     | SubstrateQueryTerm t0 -> *)
+(* 	    let res =  *)
+(*           FStarTermOfITerm *)
+(*             (TypeHeaders.substrateQueryTerm_apply t0   *)
+(* 		       (\* not sure why I need the TypeHeaders. , TypeHeaders has been opened *\) *)
+(* 		       (TranslationFromFStar.ISubstitutionOfFStarSubstitution s) ) *)
+(* 		in let _ = Assume <(res = (Subst i s))> () in *)
+(* 		res *)
+	
+(*     | SubstrateUpdateTerm t0 -> *)
+(* 	    let res = *)
+(*           FStarTermOfITerm  *)
+(*             (TypeHeaders.substrateUpdateTerm_apply t0  *)
+(* 		       (TranslationFromFStar.ISubstitutionOfFStarSubstitution s) ) *)
+(* 		in let _ = Assume <(res = (Subst i s))> () in *)
+(* 		res *)
+	
+(*     | ConcretizationEvidence t1 s1 -> raise "Evidences not handled" *)
+(* 	  (\* ConcretizationEvidence (ConcretizationEvidence t1 s1) s *\) (\* correct?? *\) *)
+(*       (\* Types.ConcretizationEvidence t1 (composeWith s s1) *\) *)
+
+and substList ilist s = match ilist with
+  | [] -> []
+  | hd::tl -> 
+      let tl' = substList tl s in 
+      let hd' = subst hd s in
+        Cons<term>  hd' tl' (* type inference is too eager here; need to provide explicit annotation on Cons *)
