ModularEngine/src/LogicEngine.FStar/typing.fst
@@ -1,0 +1,195 @@
+module Typing
+open Types
+open Util
+
+(* 1. Dynamic type tests from .NET *)
+type TypeOf :: object => typ => E
+val check_object_typ : x:object -> t:typ -> b:bool{b=true => TypeOf x t}
+
+(* judgment: is l a list of just constants c *)
+type ConstList :: 'a::* => 'a => list 'a => P =
+  | ConstList_Nil : 'a::* -> c:'a -> ConstList 'a c []
+  | ConstList_Cons : 'a::* -> c:'a -> t:list 'a
+                   -> ConstList 'a c t
+                   -> ConstList 'a c (c::t)
+val constList: c:'a -> l:list 'a -> option(ConstList c l)
+let rec constList c = function
+  | [] -> Some(ConstList_Nil c)
+  | h::t when h = c -> 
+      (match constList c t with
+         | None -> None
+         | Some p -> Some(ConstList_Cons c t p))
+  | _ -> None
+
+type WF :: substrate => infostrate => varDecl => P 
+val checkWF : s:substrate -> k:infostrate -> g:varDecl -> option (WF s k g)
+(* TODO, i.e., unique names in vardecl *)
+
+(* NS: Can we write this as a logic function? *)
+type FuncTyping :: f:func => typArgs:list typ => typRes:typ => P =
+  (* 5 with variable number of arguments *)
+  | FuncTyping_SeqRule : l:list typ -> ConstList RuleT l 
+                      -> FuncTyping SeqRule l RuleT
+  | FuncTyping_SeqCondition : l:list typ -> ConstList Condition l 
+                           -> FuncTyping SeqCondition l Condition
+  | FuncTyping_SeqAction : l:list typ -> ConstList Action l
+                        -> FuncTyping SeqAction l Action
+  | FuncTyping_AndInfon : l:list typ -> ConstList Infon l
+                       -> FuncTyping AndInfon l Infon
+  | FuncTyping_AndEvidence : l:list typ -> ConstList Evidence l
+                       -> FuncTyping AndEvidence l Evidence
+  (* all others *)
+  | FuncTyping_EmptyRule : FuncTyping EmptyRule [] RuleT
+  | FuncTyping_Rule : FuncTyping Rule [Condition; Action] RuleT
+  | FuncTyping_RuleOnce : FuncTyping RuleOnce [Condition; Action] RuleT
+  | FuncTyping_EmptyCondition : FuncTyping EmptyCondition [] Condition
+  | FuncTyping_WireCondition : FuncTyping WireCondition [Infon; Principal] Condition
+  | FuncTyping_KnownCondition : FuncTyping KnownCondition [Infon] Condition
+  | FuncTyping_EmptyAction : FuncTyping EmptyAction [] Action
+  | FuncTyping_Send : FuncTyping Send [Principal; Infon] Action
+  | FuncTyping_JustifiedSend : FuncTyping JustifiedSend [Principal; Infon] Action
+  | FuncTyping_JustifiedSay : FuncTyping JustifiedSay [Principal; Infon] Action
+  | FuncTyping_Learn : FuncTyping Learn [Infon] Action
+  | FuncTyping_Forget : FuncTyping Forget [Infon] Action
+  | FuncTyping_Install : FuncTyping Install [RuleT] Action
+  | FuncTyping_Uninstall : FuncTyping Uninstall [RuleT] Action
+  | FuncTyping_Apply : FuncTyping Apply [SubstrateUpdate] Action
+  | FuncTyping_Drop : FuncTyping Drop [Infon] Action
+  | FuncTyping_EmptyInfon : FuncTyping EmptyInfon [] Infon
+  | FuncTyping_AsInfon : FuncTyping AsInfon [SubstrateQuery] Infon
+  | FuncTyping_ImpliesInfon : FuncTyping ImpliesInfon [Infon; Infon] Infon
+  | FuncTyping_SaidInfon : FuncTyping SaidInfon [Principal; Infon] Infon
+  | FuncTyping_JustifiedInfon : FuncTyping JustifiedInfon [Infon; Evidence] Infon
+  | FuncTyping_EmptyEvidence : FuncTyping EmptyEvidence [] Evidence
+  | FuncTyping_SignatureEvidence : FuncTyping SignatureEvidence 
+      [Principal; Infon; Int32] Evidence
+  | FuncTyping_ModusPonensEvidence : FuncTyping ModusPonensEvidence 
+      [Evidence; Evidence] Evidence
+  | FuncTyping_AsInfonEvidence : FuncTyping AsInfonEvidence [SubstrateQuery] Evidence
+  | FuncTyping_RelationInfon : r:relationInfon 
+                  -> FuncTyping (RelationInfon r) r.argsType r.retType
+
+val funcTyping : f:func -> typArgs:list typ 
+              -> option (typRes:typ * FuncTyping f typArgs typRes)
+let funcTyping f typArgs = 
+  let getTyp = function (* it's also the return type *)
+    | SeqRule -> RuleT, RuleT
+    | SeqCondition -> Condition, Condition
+    | SeqAction -> Action, Action
+    | AndInfon -> Infon, Infon
+    | AndEvidence -> Evidence, Evidence in
+  match f, typArgs with
+  (* 5 with variable number of arguments *)
+  (*| (SeqRule, l) | (SeqCondition, l) | (SeqAction, l) (* Rk: no multiple match? *)
+  | (AndInfon, l) | (AndEvidence, l) -> *)
+  (* Rk: in conditions, = seems to bind tighter than || *)
+  | SeqRule, _ -> 
+      (match constList RuleT typArgs with
+       | None -> None
+       | Some c -> Some((RuleT, FuncTyping_SeqRule typArgs c)))
+  | SeqCondition, _ -> 
+      (match constList Condition typArgs with
+       | None -> None
+       | Some c -> Some((Condition, FuncTyping_SeqCondition typArgs c)))
+  | SeqAction, _ -> 
+      (match constList Action typArgs with
+       | None -> None
+       | Some c -> Some((Action, FuncTyping_SeqAction typArgs c)))
+  | AndInfon, _ -> 
+      (match constList Infon typArgs with
+       | None -> None
+       | Some c -> Some((Infon, FuncTyping_AndInfon typArgs c)))
+  | AndEvidence, _ -> 
+      (match constList Evidence typArgs with
+       | None -> None
+       | Some c -> Some((Evidence, FuncTyping_AndEvidence typArgs c)))
+  (* all others *)
+  | EmptyRule, [] -> Some((RuleT, FuncTyping_EmptyRule))
+  | Rule, [Condition; Action] -> Some((RuleT, FuncTyping_Rule))
+  | RuleOnce, [Condition; Action]-> Some((RuleT, FuncTyping_RuleOnce))
+  | EmptyCondition, []-> Some((Condition, FuncTyping_EmptyCondition))
+  | WireCondition, [Infon; Principal]-> Some((Condition, FuncTyping_WireCondition))
+  | KnownCondition, [Infon]-> Some((Condition, FuncTyping_KnownCondition))
+  | EmptyAction, []-> Some((Action, FuncTyping_EmptyAction))
+  | Send, [Principal; Infon]-> Some((Action, FuncTyping_Send))
+  | JustifiedSend, [Principal; Infon]-> Some((Action, FuncTyping_JustifiedSend))
+  | JustifiedSay, [Principal; Infon]-> Some((Action, FuncTyping_JustifiedSay))
+  | Learn, [Infon] -> Some((Action, FuncTyping_Learn))
+  | Forget, [Infon]-> Some((Action, FuncTyping_Forget))
+  | Install, [RuleT]-> Some((Action, FuncTyping_Install))
+  | Uninstall, [RuleT]-> Some((Action, FuncTyping_Uninstall))
+  | Apply, [SubstrateUpdate]-> Some((Action, FuncTyping_Apply))
+  | Drop, [Infon]-> Some((Action, FuncTyping_Drop))
+  | EmptyInfon, [] -> Some((Infon, FuncTyping_EmptyInfon))
+  | AsInfon, [SubstrateQuery]-> Some((Infon, FuncTyping_AsInfon))
+  | ImpliesInfon, [Infon; Infon]-> Some((Infon, FuncTyping_ImpliesInfon))
+  | SaidInfon, [Principal; Infon]-> Some((Infon, FuncTyping_SaidInfon))
+  | JustifiedInfon, [Infon; Evidence]-> Some((Infon, FuncTyping_JustifiedInfon))
+  | EmptyEvidence, []-> Some((Evidence, FuncTyping_EmptyEvidence))
+  | SignatureEvidence, [Principal; Infon; Int32]-> 
+      Some((Evidence, FuncTyping_SignatureEvidence))
+  | ModusPonensEvidence, [Evidence; Evidence]-> 
+      Some((Evidence, FuncTyping_ModusPonensEvidence))
+  | AsInfonEvidence, [SubstrateQuery]-> 
+      Some((Evidence, FuncTyping_AsInfonEvidence))
+  | RelationInfon r, a when a = r.argsType -> 
+      Some((r.retType, FuncTyping_RelationInfon r))
+
+type types :: varDecl => term => typ => P =
+  | Types_Var : G:varDecl
+               -> v:var
+               -> Mem v G
+               -> types G (Var v) v.typ
+               (* TODO: change rules for name clashes/scope *)
+  | Types_ConstTrueT : G:varDecl -> types G (Const TrueT) Boolean
+  | Types_ConstFalseT : G:varDecl -> types G (Const FalseT) Boolean
+  | Types_ConstPrincipalConstant : G:varDecl -> p:principal
+                             -> types G (Const (PrincipalConstant p)) Principal
+  | Types_ConstSubstrateConstant : G:varDecl -> t:typ -> o:object{TypeOf o t}
+                                 -> types G (Const (SubstrateConstant o)) t
+  | Types_ForallT : G:varDecl -> x:var -> i:term
+                   -> types (x::G) i Infon
+                   -> types G (ForallT x i) Infon
+  (*??: is this rule really true? *)
+  | Types_SubstrateQueryTerm : G:varDecl -> q:ISubstrateQueryTerm 
+                               (* TODO: check this rule *)
+                               -> types G (SubstrateQueryTerm q) SubstrateQuery
+  (* generic App rule that replaces all the others *)
+  | Types_App : g:varDecl 
+             -> f:func
+             -> args:list term
+             -> typArgs: list typ
+             -> typRes: typ
+             -> Zip term typ (types g) args typArgs
+             (*-> Zip (fun i t -> types g i t) ilist tylist*) (* ask Nik difference *)
+             -> FuncTyping f typArgs typRes
+             -> types g (App f args) typRes
+
+
+val doType: g:varDecl -> t:term -> option(ty:typ * (types g t ty))
+let rec doType g = function
+  | Var v -> (match mem v g with (* TODO: change with new rules *)
+                | None -> None
+                | Some m -> Some((v.typ, Types_Var g v m)))
+  | Const TrueT -> Some((Boolean, Types_ConstTrueT g))
+  | Const FalseT -> Some((Boolean, Types_ConstFalseT g))
+  | Const(PrincipalConstant p) ->
+      Some((Principal,
+            Types_ConstPrincipalConstant g p))
+  | ForallT x i -> (match doType (x::g) i with
+                     | None -> None
+                     | Some((Infon, pr)) ->
+                         Some((Infon, Types_ForallT g x i pr))
+                     | Some _ -> None)
+  | SubstrateQueryTerm q -> Some(SubstrateQuery, Types_SubstrateQueryTerm g q)
+  | App f args -> 
+     (match map_p_opt (doType g) args with
+        | None -> None
+        | Some((typArgs, przip)) ->
+           (match funcTyping f typArgs with
+              | None -> None
+              | Some((typRes, fpr)) ->
+                   Some((typRes, 
+				         Types_App g f args typArgs typRes przip fpr))))
+  | _ -> None
+
